# Practice Problems

## Algebra
1. Solve $ 2x^2 - 3x - 5 = 0 $.
2. Factorize $ x^2 + 7x + 10 $.
3. Simplify $ \frac{3x^2 - 2x}{x^2 - 4} $.
4. Expand and simplify $ (x + 3)(x - 4) $.
5. Solve for $ x $: $ \frac{2}{x + 1} = 3 $.

## Functions and Graphs
1. Sketch the graph of $ y = 2x^2 - 3x + 1 $.
2. Find the inverse of the function $ f(x) = \frac{3x - 5}{2} $.
3. For $ f(x) = 2x + 1 $, find the value of $ f(3) $.
4. Determine the domain and range of $ f(x) = \sqrt{x-2} $.
5. Find the turning points of the function $ y = x^3 - 3x^2 + 2x $.

## Trigonometry
1. Solve $ \sin \theta = \frac{1}{2} $ for $ 0^\circ \leq \theta < 360^\circ $.
2. Prove the identity: $ \sin^2 \theta + \cos^2 \theta = 1 $.
3. Find the exact value of $ \tan 45^\circ $.
4. Solve $ \cos \theta = -\frac{1}{2} $ for $ 0^\circ \leq \theta < 360^\circ $.
5. Solve $ \sin(\theta) = \frac{\sqrt{3}}{2} $ for $ 0 \leq \theta < 2\pi $ (in radians).

## Sequences and Series
1. Find the 10th term of the arithmetic sequence: $ 2, 5, 8, 11, \dots $.
2. Calculate the sum of the first 15 terms of the geometric series: $ 3, 6, 12, 24, \dots $.
3. The nth term of a sequence is given by $ a_n = 4n - 1 $. Find the 20th term.
4. Find the sum of the infinite geometric series $ 1 + \frac{1}{2} + \frac{1}{4} + \dots $.
5. If the first term of an arithmetic sequence is 5 and the common difference is 3, find the sum of the first 20 terms.

## Coordinate Geometry
1. Find the equation of the line passing through the points $ (2, 3) $ and $ (4, 7) $.
2. What is the distance between the points $ (1, 2) $ and $ (4, 6) $?
3. Find the midpoint of the line segment joining $ (-3, 2) $ and $ (5, -4) $.
4. Find the equation of the line parallel to $ 3x - 4y = 12 $ that passes through the point $ (1, 2) $.
5. Find the area of the triangle with vertices at $ (1, 2) $, $ (3, 4) $, and $ (5, 0) $.

## Probability
1. A bag contains 5 red balls and 3 blue balls. What is the probability of drawing a red ball?
2. Two dice are rolled. What is the probability of getting a sum of 8?
3. A deck of cards contains 52 cards. What is the probability of drawing a queen?
4. A coin is flipped three times. What is the probability of getting exactly two heads?
5. A box contains 10 marbles: 4 red, 3 blue, and 3 green. If one marble is drawn at random, what is the probability it is either red or green?

## Solving Linear Equations
1. Solve $ 3x - 5 = 16 $.
2. Solve the system of equations: 
    ```{math}
    2x + y = 7 \quad \text{and} \quad x - y = 1.
    ```
3. Solve for $ x $: $ 5x + 3 = 2x + 12 $.
4. Solve the system of equations:
    ```{math}
    4x - 2y = 10 \quad \text{and} \quad 3x + y = 9.
    ```
5. Solve $ 2(x - 1) = 3(x + 2) - 4 $.

## Partial Fractions, Remainder Theorem, and Algebraic Fractions
1. Express $ \frac{3x + 5}{(x - 1)(x + 2)} $ as the sum of partial fractions.
2. Use the remainder theorem to find the remainder when $ x^3 - 4x^2 + 3x - 2 $ is divided by $ x - 1 $.
3. Simplify $ \frac{x^2 + 5x + 6}{x^2 - 1} $.
4. Find the value of the constant $ k $ such that $ \frac{x^2 + 2x + k}{x + 1} $ has a remainder of 5 when divided by $ x + 1 $.
5. Use long division to divide $ \frac{x^3 - 2x^2 + 3x - 4}{x - 1} $ and find the quotient and remainder.


# Practice Problem Solutions
## Algebra

1. Solve $ 3x - 5 = 16 $:
```{math}
3x = 21 \quad \Rightarrow \quad x = 7.
```

2. Solve the system of equations:
```{math}
2x + y = 7 \quad \text{and} \quad x - y = 1.
```
Add the equations:
```{math}
(2x + y) + (x - y) = 7 + 1 \quad \Rightarrow \quad 3x = 8 \quad \Rightarrow \quad x = \frac{8}{3}.
```
Substitute $ x = \frac{8}{3} $ into $ 2x + y = 7 $:
```{math}
2\left(\frac{8}{3}\right) + y = 7 \quad \Rightarrow \quad \frac{16}{3} + y = 7 \quad \Rightarrow \quad y = 7 - \frac{16}{3} = \frac{5}{3}.
```

3. Solve for $ x $: $ 5x + 3 = 2x + 12 $:
```{math}
3x = 9 \quad \Rightarrow \quad x = 3.
```

4. Solve the system of equations:
```{math}
4x - 2y = 10 \quad \text{and} \quad 3x + y = 9.
```
Multiply the second equation by 2:
```{math}
6x + 2y = 18.
```
Add the equations:
```{math}
(4x - 2y) + (6x + 2y) = 10 + 18 \quad \Rightarrow \quad 10x = 28 \quad \Rightarrow \quad x = \frac{28}{10} = 2.8.
```
Substitute $ x = 2.8 $ into $ 3x + y = 9 $:
```{math}
3(2.8) + y = 9 \quad \Rightarrow \quad 8.4 + y = 9 \quad \Rightarrow \quad y = 0.6.
```

5. Solve $ 2(x - 1) = 3(x + 2) - 4 $:
```{math}
2x - 2 = 3x + 6 - 4 \quad \Rightarrow \quad 2x - 2 = 3x + 2 \quad \Rightarrow \quad -2 = x + 2 \quad \Rightarrow \quad x = -4.
```

---

## Functions

1. Find the range of $ f(x) = 2x + 3 $ when $ x $ is in the set $ \{1, 2, 3\} $:
For $ x = 1 $: $ f(1) = 2(1) + 3 = 5 $.

For $ x = 2 $: $ f(2) = 2(2) + 3 = 7 $.

For $ x = 3 $: $ f(3) = 2(3) + 3 = 9 $.

Thus, the range is $ \{5, 7, 9\} $.

2. Solve $ f(x) = 0 $ for $ f(x) = 3x^2 - 5x + 2 $:
```{math}
3x^2 - 5x + 2 = 0.
```
Use the quadratic formula:
```{math}
x = \frac{-(-5) \pm \sqrt{(-5)^2 - 4(3)(2)}}{2(3)} = \frac{5 \pm \sqrt{25 - 24}}{6} = \frac{5 \pm \sqrt{1}}{6} = \frac{5 \pm 1}{6}.
```
Thus, $ x = \frac{6}{6} = 1 $ or $ x = \frac{4}{6} = \frac{2}{3} $.

3. Find the domain of $ f(x) = \frac{1}{x-2} $:
The domain is all real numbers except $ x = 2 $, where the denominator is zero. Thus, the domain is $ x \in \mathbb{R} \setminus \{2\} $.

4. Find the inverse of $ f(x) = 2x + 1 $:
To find the inverse, swap $ x $ and $ y $ and solve for $ y $:
```{math}
x = 2y + 1 \quad \Rightarrow \quad x - 1 = 2y \quad \Rightarrow \quad y = \frac{x - 1}{2}.
```
Thus, the inverse is $ f^{-1}(x) = \frac{x - 1}{2} $.

5. Solve $ f(x) = 4 $ for $ f(x) = x^2 - 3x + 2 $:
```{math}
x^2 - 3x + 2 = 4 \quad \Rightarrow \quad x^2 - 3x - 2 = 0.
```
Factor the quadratic:
```{math}
(x - 2)(x - (-1)) = 0.
```
Thus, $ x = 2 $ or $ x = -1 $.

---

## Trigonometry

1. Solve $ \sin x = \frac{1}{2} $ for $ 0^\circ \leq x \leq 360^\circ $:
The solutions are $ x = 30^\circ $ and $ x = 150^\circ $.

2. Find the exact value of $ \cos 45^\circ $:
```{math}
\cos 45^\circ = \frac{\sqrt{2}}{2}.
```

3. Find the period of $ f(x) = \sin(3x) $:
The period of $ f(x) = \sin(kx) $ is $ \frac{360^\circ}{k} $, so for $ k = 3 $, the period is:
```{math}
\frac{360^\circ}{3} = 120^\circ.
```

4. Solve $ \tan x = 1 $ for $ 0^\circ \leq x \leq 360^\circ $:
The solutions are $ x = 45^\circ $ and $ x = 225^\circ $.

5. Find $ \sin \theta $ if $ \theta = 60^\circ $ (radians):
```{math}
\theta = 60^\circ = \frac{\pi}{3} \text{ radians}.
```

```{math}
\sin\left( \frac{\pi}{3} \right) = \frac{\sqrt{3}}{2}.
```

---

## Geometry

1. Find the distance between the points $ (1, 2) $ and $ (4, 6) $:
```{math}
d = \sqrt{(4 - 1)^2 + (6 - 2)^2} = \sqrt{9 + 16} = \sqrt{25} = 5.
```

2. Find the midpoint of the line segment joining $ (-3, 2) $ and $ (5, -4) $:
```{math}
\text{Midpoint} = \left( \frac{-3 + 5}{2}, \frac{2 + (-4)}{2} \right) = (1, -1).
```

3. Find the equation of the line parallel to $ 3x - 4y = 12 $ that passes through the point $ (1, 2) $:
Rearranging $ 3x - 4y = 12 $ gives $ y = \frac{3}{4}x - 3 $. The slope is $ \frac{3}{4} $.
Using the point-slope form:
```{math}
y - 2 = \frac{3}{4}(x - 1) \quad \Rightarrow \quad y = \frac{3}{4}x + \frac{5}{4}.
```

4. Find the area of the triangle with vertices at $ (1, 2) $, $ (3, 4) $, and $ (5, 0) $:
Using the area formula for a triangle with vertices $ (x_1, y_1) $, $ (x_2, y_2) $, and $ (x_3, y_3) $:
```{math}
\text{Area} = \frac{1}{2} \left| x_1(y_2 - y_3) + x_2(y_3 - y_1) + x_3(y_1 - y_2) \right|
```
```{math}
= \frac{1}{2} \left| 1(4 - 0) + 3(0 - 2) + 5(2 - 4) \right| = \frac{1}{2} \left| 4 - 6 - 10 \right| = \frac{1}{2} \times 12 = 6.
```

5. Find the circumference of a circle with radius 7 cm:
```{math}
C = 2\pi r = 2\pi \times 7 = 14\pi \text{ cm}.
```

---

## Statistics

1. Find the mean of the data set $ 3, 7, 8, 5, 10 $:
```{math}
\text{Mean} = \frac{3 + 7 + 8 + 5 + 10}{5} = \frac{33}{5} = 6.6.
```

2. Calculate the median of the data set $ 4, 1, 7, 3, 6 $:
Sort the data: $ 1, 3, 4, 6, 7 $. The median is the middle value:
```{math}
\text{Median} = 4.
```

3. Find the mode of the data set $ 2, 4, 4, 6, 7, 7, 7 $:
The mode is the most frequent number:
```{math}
\text{Mode} = 7.
```

4. Find the standard deviation of the data set $ 2, 4, 6, 8 $:
First, find the mean:
```{math}
\text{Mean} = \frac{2 + 4 + 6 + 8}{4} = 5.
```
Then, find the squared differences from the mean:
```{math}
(2 - 5)^2 = 9, \quad (4 - 5)^2 = 1, \quad (6 - 5)^2 = 1, \quad (8 - 5)^2 = 9.
```
The variance is the average of these squared differences:
```{math}
\text{Variance} = \frac{9 + 1 + 1 + 9}{4} = 5.
```
Thus, the standard deviation is:
```{math}
\text{Standard Deviation} = \sqrt{5} \approx 2.24.
```

5. Find the probability of drawing a red card from a standard deck of cards:
There are 52 cards in total, with 26 red cards (hearts and diamonds):
```{math}
\text{Probability} = \frac{26}{52} = \frac{1}{2}.
```

---

## Sequences and Series

1. Find the 5th term of the arithmetic sequence: $ 2, 5, 8, 11, \dots $:
The common difference is 3. The nth term formula is:
```{math}
a_n = a_1 + (n-1) \times d.
```
For the 5th term:
```{math}
a_5 = 2 + (5-1) \times 3 = 2 + 12 = 14.
```

2. Find the sum of the first 6 terms of the geometric sequence: $ 3, 6, 12, 24, \dots $:
The first term is $ a_1 = 3 $ and the common ratio is $ r = 2 $. The sum of the first $ n $ terms of a geometric sequence is:
```{math}
S_n = \frac{a_1(1 - r^n)}{1 - r}.
```
For $ n = 6 $:
```{math}
S_6 = \frac{3(1 - 2^6)}{1 - 2} = \frac{3(1 - 64)}{-1} = \frac{3 \times (-63)}{-1} = 189.
```

3. Find the 10th term of the Fibonacci sequence:
The Fibonacci sequence is defined by $ F_1 = 1 $, $ F_2 = 1 $, and $ F_n = F_{n-1} + F_{n-2} $.
The first 10 terms are:
```{math}
1, 1, 2, 3, 5, 8, 13, 21, 34, 55.
```
Thus, the 10th term is $ 55 $.

4. Find the sum of the first 8 terms of the arithmetic sequence: $ 4, 8, 12, 16, \dots $:
The first term is $ a_1 = 4 $ and the common difference is $ d = 4 $. The sum of the first $ n $ terms is:
```{math}
S_n = \frac{n}{2} \times (2a_1 + (n-1) \times d).
```
For $ n = 8 $:
```{math}
S_8 = \frac{8}{2} \times (2 \times 4 + (8-1) \times 4) = 4 \times (8 + 28) = 4 \times 36 = 144.
```

5. Find the sum of the first 5 terms of the geometric sequence: $ 1, 3, 9, 27, \dots $:
The first term is $ a_1 = 1 $ and the common ratio is $ r = 3 $. The sum of the first $ n $ terms is:
```{math}
S_n = \frac{a_1(1 - r^n)}{1 - r}.
```
For $ n = 5 $:
```{math}
S_5 = \frac{1(1 - 3^5)}{1 - 3} = \frac{1(1 - 243)}{-2} = \frac{-242}{-2} = 121.
```

---

## Partial Fractions, Remainder Theorem, and Algebraic Fractions

1.  Decompose $ \frac{5x + 3}{x^2 + 2x - 3} $ into partial fractions:
Factor the denominator:
```{math}
x^2 + 2x - 3 = (x - 1)(x + 3).
```
Write the partial fraction decomposition:
```{math}
\frac{5x + 3}{(x - 1)(x + 3)} = \frac{A}{x - 1} + \frac{B}{x + 3}.
```
Multiply both sides by $ (x - 1)(x + 3) $:
```{math}
5x + 3 = A(x + 3) + B(x - 1).
```
Expanding both sides:
```{math}
5x + 3 = (A + B)x + (3A - B).
```
Equate the coefficients of $ x $ and the constant term:
```{math}
A + B = 5 \quad \text{and} \quad 3A - B = 3.
```
Solve the system of equations:
```{math}
A = 2, \quad B = 3.
```
Thus, the partial fraction decomposition is:
```{math}
\frac{5x + 3}{(x - 1)(x + 3)} = \frac{2}{x - 1} + \frac{3}{x + 3}.
```

2. Use the remainder theorem to find the remainder when $ f(x) = 3x^3 + 2x^2 - 5x + 4 $ is divided by $ x - 2 $:
The remainder is $ f(2) $:
```{math}
f(2) = 3(2)^3 + 2(2)^2 - 5(2) + 4 = 3(8) + 2(4) - 10 + 4 = 24 + 8 - 10 + 4 = 26.
```
The remainder is $ 26 $.

3. Simplify the expression $ \frac{x^2 + 2x - 3}{x^2 + x - 6} $:
Factor the numerator and denominator:
```{math}
\frac{x^2 + 2x - 3}{x^2 + x - 6} = \frac{(x - 1)(x + 3)}{(x - 2)(x + 3)}.
```
Cancel the common factor $ x + 3 $:
```{math}
\frac{x - 1}{x - 2}.
```

4. Simplify the expression $ \frac{2x^2 + 5x - 3}{x^2 + 4x - 5} $:
Factor the numerator and denominator:
```{math}
\frac{2x^2 + 5x - 3}{x^2 + 4x - 5} = \frac{(2x - 1)(x + 3)}{(x - 1)(x + 5)}.
```

5. Perform polynomial long division: $ \frac{3x^2 - 5x + 2}{x - 2} $:

1. Divide the leading term $ 3x^2 $ by $ x $: $ 3x $.
2. Multiply $ 3x $ by $ x - 2 $: $ 3x^2 - 6x $.
3. Subtract $ (3x^2 - 6x) $ from $ 3x^2 - 5x + 2 $: $ x + 2 $.
4. Divide $ x $ by $ x $: $ 1 $.
5. Multiply $ 1 $ by $ x - 2 $: $ x - 2 $.
6. Subtract $ (x - 2) $ from $ x + 2 $: $ 4 $.

Thus, the quotient is $ 3x + 1 $ and the remainder is $ 4 $, so:
```{math}
\frac{3x^2 - 5x + 2}{x - 2} = 3x + 1 + \frac{4}{x - 2}.
\}

